\documentclass{article}
\usepackage{fancyhdr}
\usepackage{amsmath}
\usepackage{amsthm}
\usepackage{accents}
\usepackage{amssymb}
\usepackage{graphicx}
\usepackage{float}
\usepackage{subcaption}
\usepackage{hyperref}
\usepackage{listings}
\usepackage{color}
\usepackage{tikz}
\usepackage{pgfplots}
\usepackage{pgfplotstable}
\usepackage{listings}
\usepackage{color}
\usepackage{tikz}
\usepackage{amsthm}
\usepackage{soul}
\usepackage[margin=15mm]{geometry}

\definecolor{dkgreen}{rgb}{0,0.6,0}
\definecolor{gray}{rgb}{0.5,0.5,0.5}
\definecolor{mauve}{rgb}{0.58,0,0.82}
\hypersetup{colorlinks=true,linkcolor=blue, linktocpage}
% Set up fancy header
\pagestyle{fancy}
\fancyhf{} % Clear default header and footer
\rhead{Keith Wesa} % Right header
\lhead{CS 151 Homework 2:} % Left header
\rfoot{Page \thepage} % Right footer

\author{Keith Wesa}
\title{MAT 215 - Written Homework 1}
\date{\today}

\begin{document}
\section*{Question 1.3}
\subsection*{The problem}
\begin{itemize}
    \item[Q1.3] Every dog runs or eats. Every dog that eats but doesn't run, sleeps.
    Therefore, every dog that doesn't sleep, runs.
    \item[] Let $R(x)$ be "x runs", $E(x)$ be "x eats", $S(x)$ be "x sleeps", the domain of $x$ consists of all dogs.
    \item[] \textbf{Compound Logic Form: } $(\forall x ((R(x) \lor E(x))) \land \forall x ((E(x) \land \neg R(x)) \rightarrow S(x))) \rightarrow \forall x (\neg S(x) \rightarrow R(x))$
    \item[] \textbf{Argument Form:}
    \begin{equation*}
        \begin{aligned}
            &\forall x ((R(x) \lor E(x))) \\
            &\forall x ((E(x) \land \neg R(x)) \rightarrow S(x)) \\
            \hline
            &\therefore \forall x (\neg S(x) \rightarrow R(x))
        \end{aligned}
    \end{equation*}
    \item[] \textbf{Validate Argument:}
     \begin{proof}
        \begin{align*}
            &\forall x ((R(x) \lor E(x))) \tag{Hypothesis} \\
            &\forall x ((E(x) \land \neg R(x)) \rightarrow S(x)) \tag{Hypothesis} \\
            &\forall x (\neg S(x) \rightarrow R(x)) \tag{Conclusion} \\
            &\text{Let } x \text{ be an arbitrary dog} \\
            &\text{Assume } \neg S(x) \tag{Assumption} \\
            &\text{Assume } \neg R(x) \tag{Assumption} \\
            &E(x) \land \neg R(x) \tag{Conjunction Introduction} \\
            &E(x) \land \neg R(x) \rightarrow S(x) \tag{Universal Instantiation} \\
            &S(x) \tag{Modus Ponens} \\
            &\neg S(x) \land S(x) \tag{Conjunction} \\
            &\neg \neg R(x) \tag{Negation} \\
            &R(x) \tag{Double Negation} \\
            &\neg S(x) \rightarrow R(x) \tag{Conditional} \\
            &\forall x (\neg S(x) \rightarrow R(x)) \tag{Universal Instantiation} \\
            &\boxed { \therefore \forall x (\neg S(x) \rightarrow R(x))} \tag{Conclusion} 
        \end{align*}
    \end{proof}       
\end{itemize}
\end{document}